Much more progress

Data/Alternative.hs
@@ -1,0 +1,27 @@
+module Data.Alternative where
+
+import qualified Prelude
+import qualified Data.List
+import qualified Data.Applicative as Applicative
+
+
+__ :: any
+__ = Prelude.error "Logical or arity value used"
+
+data Alternative f =
+   Build_Alternative (Applicative.Applicative f) (() -> f) (() -> f -> f ->
+                                                           f)
+
+choose :: (Alternative a1) -> a1 -> a1 -> a1
+choose alternative x x0 =
+  case alternative of {
+   Build_Alternative alt_is_applicative empty choose0 -> choose0 __ x x0}
+
+option_Alternative :: Alternative (Prelude.Maybe ())
+option_Alternative =
+  Build_Alternative Applicative.option_Applicative (\_ -> Prelude.Nothing)
+    (\_ x y ->
+    case x of {
+     Prelude.Just wildcard' -> x;
+     Prelude.Nothing -> y})
+
