Data/Applicative.hs
@@ -1,0 +1,40 @@
+{-# OPTIONS_GHC -cpp -fglasgow-exts #-}
+{- For Hugs, use the option -F"cpp -P -traditional" -}
+
+module Data.Applicative where
+
+import qualified Prelude
+import qualified Data.List
+import qualified Data.Endo as Endo
+
+
+
+--unsafeCoerce :: a -> b
+#ifdef __GLASGOW_HASKELL__
+import qualified GHC.Base as GHC.Base
+unsafeCoerce = GHC.Base.unsafeCoerce#
+#else
+-- HUGS
+import qualified Data.IOExts as IOExts
+unsafeCoerce = IOExts.unsafeCoerce
+#endif
+
+__ :: any
+__ = Prelude.error "Logical or arity value used"
+
+data Applicative f =
+   Build_Applicative (Endo.Functor f) (() -> () -> f) (() -> () -> f -> f ->
+                                                      f)
+
+option_Applicative :: Applicative (Prelude.Maybe ())
+option_Applicative =
+  Build_Applicative Endo.option_Functor
+    (unsafeCoerce (\_ x -> Prelude.Just x)) (\_ _ f x ->
+    case f of {
+     Prelude.Just f' ->
+      unsafeCoerce (\f'0 _ ->
+        case x of {
+         Prelude.Just x' -> Prelude.Just (f'0 x');
+         Prelude.Nothing -> Prelude.Nothing}) f' __;
+     Prelude.Nothing -> Prelude.Nothing})
+
