Data/Interval.hs
@@ -1,12 +1,28 @@
+{-# OPTIONS_GHC -cpp -fglasgow-exts #-}
+{- For Hugs, use the option -F"cpp -P -traditional" -}
+
 module Data.Interval where
 
 import qualified Prelude
 import qualified Data.List
+import qualified Data.Alternative as Alternative
+import qualified Data.Endo as Endo
 import qualified Data.NPeano as NPeano
 import qualified Data.NonEmpty0 as NonEmpty0
 import qualified Data.Peano as Peano
 import qualified Data.Range as Range
 
+
+
+--unsafeCoerce :: a -> b
+#ifdef __GLASGOW_HASKELL__
+import qualified GHC.Base as GHC.Base
+unsafeCoerce = GHC.Base.unsafeCoerce#
+#else
+-- HUGS
+import qualified Data.IOExts as IOExts
+unsafeCoerce = IOExts.unsafeCoerce
+#endif
 
 data IntervalDesc =
    Build_IntervalDesc Prelude.Int Prelude.Int (NonEmpty0.NonEmpty
@@ -44,16 +60,16 @@ intervalExtent :: IntervalDesc -> Prelude.Int
 intervalExtent d =
   Peano.minus (intervalEnd d) (intervalStart d)
 
-anyRangeIntersects :: IntervalDesc -> IntervalDesc -> Prelude.Bool
-anyRangeIntersects i j =
+intervalsIntersect :: IntervalDesc -> IntervalDesc -> Prelude.Bool
+intervalsIntersect i j =
   let {f = \x y -> Range.rangesIntersect ( x) ( y)} in
   Prelude.foldr (\r b ->
     (Prelude.||) b ((Prelude.any) (f r) (NonEmpty0.coq_NE_to_list (rds j))))
     Prelude.False (NonEmpty0.coq_NE_to_list (rds i))
 
-firstIntersectionPoint :: IntervalDesc -> IntervalDesc -> Prelude.Maybe
-                          Prelude.Int
-firstIntersectionPoint i j =
+intervalIntersectionPoint :: IntervalDesc -> IntervalDesc -> Prelude.Maybe
+                             Prelude.Int
+intervalIntersectionPoint i j =
   NonEmpty0.coq_NE_fold_left (\acc rd ->
     case acc of {
      Prelude.Just x -> Prelude.Just x;
@@ -61,6 +77,28 @@ firstIntersectionPoint i j =
       NonEmpty0.coq_NE_fold_left (\acc' rd' ->
         case acc' of {
          Prelude.Just x -> Prelude.Just x;
-         Prelude.Nothing -> Range.rangesIntersectionPoint ( rd) ( rd')})
+         Prelude.Nothing -> Range.rangeIntersectionPoint ( rd) ( rd')})
         (rds j) Prelude.Nothing}) (rds i) Prelude.Nothing
+
+findUsePos :: IntervalDesc -> (Range.UsePos -> Prelude.Bool) -> Prelude.Maybe
+              Range.UsePos
+findUsePos i f =
+  let {
+   go rs =
+     case rs of {
+      NonEmpty0.NE_Sing y -> Range.findRangeUsePos y f;
+      NonEmpty0.NE_Cons y rs' ->
+       Alternative.choose (unsafeCoerce Alternative.option_Alternative)
+         (Range.findRangeUsePos y f) (go rs')}}
+  in go (rds i)
+
+nextUseAfter :: IntervalDesc -> Prelude.Int -> Prelude.Maybe Prelude.Int
+nextUseAfter d pos =
+  Endo.fmap (unsafeCoerce Endo.option_Functor) Range.uloc
+    (unsafeCoerce (findUsePos d (\u -> NPeano.ltb pos (Range.uloc u))))
+
+firstUseReqReg :: IntervalDesc -> Prelude.Maybe Prelude.Int
+firstUseReqReg d =
+  Endo.fmap (unsafeCoerce Endo.option_Functor) Range.uloc
+    (unsafeCoerce (findUsePos d Range.regReq))
 
