Data/Range.hs
@@ -1,14 +1,39 @@
+{-# OPTIONS_GHC -cpp -fglasgow-exts #-}
+{- For Hugs, use the option -F"cpp -P -traditional" -}
+
 module Data.Range where
 
 import qualified Prelude
 import qualified Data.List
+import qualified Data.Alternative as Alternative
 import qualified Data.NPeano as NPeano
 import qualified Data.NonEmpty0 as NonEmpty0
 import qualified Data.Peano as Peano
 
 
+
+--unsafeCoerce :: a -> b
+#ifdef __GLASGOW_HASKELL__
+import qualified GHC.Base as GHC.Base
+unsafeCoerce = GHC.Base.unsafeCoerce#
+#else
+-- HUGS
+import qualified Data.IOExts as IOExts
+unsafeCoerce = IOExts.unsafeCoerce
+#endif
+
 data UsePos =
    Build_UsePos Prelude.Int Prelude.Bool
+
+uloc :: UsePos -> Prelude.Int
+uloc u =
+  case u of {
+   Build_UsePos uloc0 regReq0 -> uloc0}
+
+regReq :: UsePos -> Prelude.Bool
+regReq u =
+  case u of {
+   Build_UsePos uloc0 regReq0 -> regReq0}
 
 data RangeDesc =
    Build_RangeDesc Prelude.Int Prelude.Int (NonEmpty0.NonEmpty UsePos)
@@ -16,12 +41,17 @@ data RangeDesc =
 rbeg :: RangeDesc -> Prelude.Int
 rbeg r =
   case r of {
-   Build_RangeDesc rbeg0 rend0 ups -> rbeg0}
+   Build_RangeDesc rbeg0 rend0 ups0 -> rbeg0}
 
 rend :: RangeDesc -> Prelude.Int
 rend r =
   case r of {
-   Build_RangeDesc rbeg0 rend0 ups -> rend0}
+   Build_RangeDesc rbeg0 rend0 ups0 -> rend0}
+
+ups :: RangeDesc -> NonEmpty0.NonEmpty UsePos
+ups r =
+  case r of {
+   Build_RangeDesc rbeg0 rend0 ups0 -> ups0}
 
 rangesIntersect :: RangeDesc -> RangeDesc -> Prelude.Bool
 rangesIntersect x y =
@@ -29,10 +59,27 @@ rangesIntersect x y =
    Prelude.True -> NPeano.ltb (rbeg y) (rend x);
    Prelude.False -> NPeano.ltb (rbeg x) (rend y)}
 
-rangesIntersectionPoint :: RangeDesc -> RangeDesc -> Prelude.Maybe
-                           Prelude.Int
-rangesIntersectionPoint x y =
+rangeIntersectionPoint :: RangeDesc -> RangeDesc -> Prelude.Maybe Prelude.Int
+rangeIntersectionPoint x y =
   case rangesIntersect x y of {
    Prelude.True -> Prelude.Just (Peano.min (rbeg x) (rbeg y));
    Prelude.False -> Prelude.Nothing}
+
+findRangeUsePos :: RangeDesc -> (UsePos -> Prelude.Bool) -> Prelude.Maybe
+                   UsePos
+findRangeUsePos r f =
+  let {
+   check = \u ->
+    case f u of {
+     Prelude.True -> Prelude.Just u;
+     Prelude.False -> Prelude.Nothing}}
+  in
+  let {
+   go us =
+     case us of {
+      NonEmpty0.NE_Sing u -> check u;
+      NonEmpty0.NE_Cons u us' ->
+       Alternative.choose (unsafeCoerce Alternative.option_Alternative)
+         (check u) (go us')}}
+  in go (ups r)
 
