NonEmpty.v
@@ -1,3 +1,9 @@
+Require Import Coq.Classes.RelationClasses.
+Require Import Coq.Sorting.Sorted.
+Require Import Coq.Relations.Relations.
+
+Generalizable All Variables.
+
 (** ** NonEmpty lists *)
 
 Inductive NonEmpty (a : Set) : Set :=
@@ -13,20 +19,321 @@ Fixpoint NE_to_list {a} (ne : NonEmpty a) : list a :=
     | NE_Cons x xs => cons x (NE_to_list xs)
   end.
 
-Definition NE_hd {a} (ne : NonEmpty a) : a :=
+Definition NE_head {a} (ne : NonEmpty a) : a :=
   match ne with
     | NE_Sing x => x
     | NE_Cons x _ => x
   end.
 
-Fixpoint NE_tl {a} (ne : NonEmpty a) : a :=
+Fixpoint NE_map {a b : Set} (f : a -> b) (ne : NonEmpty a) : NonEmpty b :=
+  match ne with
+    | NE_Sing x => NE_Sing (f x)
+    | NE_Cons x xs => NE_Cons (f x) (NE_map f xs)
+  end.
+
+Fixpoint NE_last {a} (ne : NonEmpty a) : a :=
   match ne with
     | NE_Sing x => x
-    | NE_Cons x xs => NE_tl xs
+    | NE_Cons x xs => NE_last xs
   end.
+
+Lemma NE_map_head_spec : forall {a b : Set} (f : a -> b) (xs : NonEmpty a),
+  NE_head (NE_map f xs) = f (NE_head xs).
+Proof. induction xs; auto. Qed.
+
+Lemma NE_map_last_spec : forall {a b : Set} (f : a -> b) (xs : NonEmpty a),
+  NE_last (NE_map f xs) = f (NE_last xs).
+Proof. induction xs; auto. Qed.
 
 Fixpoint NE_fold_left {a b : Set} (f : a -> b -> a) (ne : NonEmpty b) (z : a) : a :=
   match ne with
     | NE_Sing x => f z x
     | NE_Cons x xs => NE_fold_left f xs (f z x)
   end.
+
+Fixpoint NE_append {a : Set} (l1 l2 : NonEmpty a) : NonEmpty a :=
+  match l1 with
+    | NE_Sing x => NE_Cons x l2
+    | NE_Cons x xs => NE_Cons x (NE_append xs l2)
+  end.
+
+Lemma NE_map_append_spec : forall {a b : Set} (f : a -> b) {xs ys : NonEmpty a},
+  NE_map f (NE_append xs ys) = NE_append (NE_map f xs) (NE_map f ys).
+Proof.
+  induction xs; intros; simpl; auto.
+  f_equal. apply IHxs.
+Qed.
+
+Lemma NE_head_append_spec : forall {a} {xs ys : NonEmpty a},
+  NE_head (NE_append xs ys) = NE_head xs.
+Proof. induction xs; auto. Qed.
+
+Lemma NE_last_append_spec : forall {a} {xs ys : NonEmpty a},
+  NE_last (NE_append xs ys) = NE_last ys.
+Proof. induction xs; auto. Qed.
+
+Fixpoint NE_span {a : Set} (f : a -> bool) (l : NonEmpty a)
+  : (option (NonEmpty a) * option (NonEmpty a)) :=
+  let maybeAppend (x : a) (xs : option (NonEmpty a)) :=
+      match xs with
+        | Some xs' => Some (NE_Cons x xs')
+        | None     => Some (NE_Sing x)
+      end in
+  match l with
+    | NE_Sing x =>
+        if f x
+        then (Some l, None)
+        else (None, Some l)
+    | NE_Cons x xs =>
+        let (xl, xr) := NE_span f xs in
+        if f x
+        then (maybeAppend x xl, xr)
+        else (xl, maybeAppend x xr)
+  end.
+
+Lemma NE_span_spec : forall a (l : NonEmpty a),
+  let (xs,ys) := NE_span (fun _ => true) l in
+  match xs with
+    | Some xs' => match ys with
+        | Some ys' => l = NE_append xs' ys'
+        | None => l = xs'
+      end
+    | None => match ys with
+        | Some ys' => l = ys'
+        | None => False
+      end
+  end.
+Proof.
+  intros.
+  induction l; simpl in *.
+    reflexivity.
+  destruct (NE_span _ l);
+  destruct o; destruct o0; simpl;
+  try (f_equal; apply IHl).
+  contradiction.
+Qed.
+
+Section Sorted.
+
+Variable A : Set.
+Variable R : relation A.
+Context `{H : Transitive A R}.
+
+Fixpoint NE_In (a : A) (l : NonEmpty A) : Prop :=
+  match l with
+    | NE_Sing b => b = a
+    | NE_Cons b m => b = a \/ NE_In a m
+  end.
+
+Inductive NE_Exists (P : A -> Prop) : NonEmpty A -> Prop :=
+ | NE_Exists_sing    : forall x,   P x -> NE_Exists P (NE_Sing x)
+ | NE_Exists_cons_hd : forall x l, P x -> NE_Exists P (NE_Cons x l)
+ | NE_Exists_cons_tl : forall x l, NE_Exists P l -> NE_Exists P (NE_Cons x l).
+
+Hint Constructors NE_Exists.
+
+Lemma NE_Exists_exists : forall P (l : NonEmpty A),
+  NE_Exists P l <-> (exists x, NE_In x l /\ P x).
+Proof.
+  split. induction 1; firstorder.
+  induction l; firstorder;
+  inversion H0; subst;
+  constructor; assumption.
+Qed.
+
+Lemma NE_Exists_cons : forall (P : A -> Prop) x l,
+  NE_Exists P (NE_Cons x l) <-> P x \/ NE_Exists P l.
+Proof. split; inversion 1; auto. Qed.
+
+Inductive NE_Forall (P : A -> Prop) : NonEmpty A -> Prop :=
+ | NE_Forall_sing : forall x, P x -> NE_Forall P (NE_Sing x)
+ | NE_Forall_cons : forall x l, P x -> NE_Forall P l -> NE_Forall P (NE_Cons x l).
+
+Hint Constructors NE_Forall.
+
+Lemma NE_Forall_forall : forall P (l : NonEmpty A),
+  NE_Forall P l <-> (forall x, NE_In x l -> P x).
+Proof.
+  split.
+    induction 1; firstorder;
+    inversion H1; subst; auto.
+  intros. induction l.
+    constructor. apply H0. constructor.
+  constructor. apply H0. constructor.
+    reflexivity.
+  apply IHl. intros.
+  apply H0. right. apply H1.
+Qed.
+
+Lemma NE_Forall_inv : forall P (a : A) l,
+  NE_Forall P (NE_Cons a l) -> P a.
+Proof. intros; inversion H0; trivial. Defined.
+
+Lemma NE_Forall_rect : forall (P : A -> Prop) (Q : NonEmpty A -> Type),
+  (forall b, P b -> Q (NE_Sing b))
+    -> (forall b l, P b -> Q (NE_Cons b l)) -> forall l, NE_Forall P l -> Q l.
+Proof.
+  intros P Q H1 H2; induction l; intro;
+  [|eapply H2, NE_Forall_inv].
+    apply H1. inversion H0. assumption.
+    apply H0.
+Defined.
+
+Lemma NE_Forall_impl : forall (P Q : A -> Prop), (forall a, P a -> Q a) ->
+  forall l, NE_Forall P l -> NE_Forall Q l.
+Proof.
+  intros P Q Himp l H1.
+  induction H1; firstorder.
+Qed.
+
+Lemma NE_Forall_head : forall x (xs : NonEmpty A),
+  NE_Forall (R x) xs -> R x (NE_head xs).
+Proof. induction xs; intros; inversion H0; assumption. Qed.
+
+Lemma NE_Forall_last : forall x (xs : NonEmpty A),
+  NE_Forall (R x) xs -> R x (NE_last xs).
+Proof.
+  intros. induction xs; simpl in *.
+    inversion H0. assumption.
+  apply IHxs. inversion H0. assumption.
+Qed.
+
+Lemma NE_Forall_append : forall (P : A -> Prop) xs ys,
+   NE_Forall P xs /\ NE_Forall P ys <-> NE_Forall P (NE_append xs ys).
+Proof.
+  split; induction xs; intros; simpl;
+  constructor; intuition;
+  try inversion H1; auto;
+  try inversion H0; auto;
+  try constructor; auto.
+  apply IHxs. assumption.
+  intuition.
+Qed.
+
+Inductive NE_StronglySorted : NonEmpty A -> Prop :=
+  | SSorted_sing a   : NE_StronglySorted (NE_Sing a)
+  | SSorted_cons a l : NE_StronglySorted l -> NE_Forall (R a) l
+                         -> NE_StronglySorted (NE_Cons a l).
+
+Lemma NE_StronglySorted_inv : forall a l, NE_StronglySorted (NE_Cons a l) ->
+  NE_StronglySorted l /\ NE_Forall (R a) l.
+Proof. intros; inversion H0; auto. Defined.
+
+Lemma NE_StronglySorted_inv_app : forall (l1 l2 : NonEmpty A),
+  NE_StronglySorted (NE_append l1 l2)
+    -> NE_StronglySorted l1 /\ NE_StronglySorted l2.
+Proof.
+  induction l1; intros; simpl; inversion H0.
+    split; [ constructor | assumption ].
+  specialize (IHl1 l2 H3).
+  inversion IHl1.
+  split.
+    constructor. assumption.
+    apply NE_Forall_append in H4. intuition.
+  assumption.
+Qed.
+
+Lemma NE_StronglySorted_rect :
+  forall P : NonEmpty A -> Type,
+    (forall a, P (NE_Sing a)) ->
+    (forall a l, NE_StronglySorted l -> P l -> NE_Forall (R a) l
+                   -> P (NE_Cons a l)) ->
+    forall l, NE_StronglySorted l -> P l.
+Proof.
+  induction l; firstorder using NE_StronglySorted_inv.
+Defined.
+
+Lemma NE_StronglySorted_rec :
+  forall P : NonEmpty A -> Type,
+    (forall a, P (NE_Sing a)) ->
+    (forall a l, NE_StronglySorted l -> P l -> NE_Forall (R a) l
+                   -> P (NE_Cons a l)) ->
+   forall l, NE_StronglySorted l -> P l.
+Proof.
+  firstorder using NE_StronglySorted_rect.
+Qed.
+
+Lemma NE_StronglySorted_Sorted : forall l,
+  NE_StronglySorted l -> Sorted R (NE_to_list l).
+Proof.
+  induction 1 as [|? ? ? ? HForall]; constructor; trivial.
+  destruct HForall; constructor; trivial.
+Qed.
+
+Lemma NE_StronglySorted_cons : forall x (xs : NonEmpty A),
+  R x (NE_head xs) -> NE_StronglySorted xs
+    -> NE_StronglySorted (NE_Cons x xs).
+Proof.
+  intros.
+  induction xs; simpl in *;
+  repeat (constructor; try assumption).
+  apply NE_StronglySorted_inv in H1. inversion H1.
+  apply NE_Forall_impl with (P := (R a)) (Q := (R x));
+    try transitivity a; assumption.
+Qed.
+
+Lemma NE_StronglySorted_cons_middle : forall x xs ys,
+  NE_StronglySorted (NE_append xs (NE_Cons x ys))
+    -> NE_StronglySorted (NE_append xs ys).
+Proof.
+  induction xs; intros; simpl in *;
+  apply NE_StronglySorted_inv in H0; inversion H0.
+    constructor;
+    inversion H1; inversion H2; assumption.
+  constructor. apply IHxs.
+    inversion H0. assumption.
+  apply NE_Forall_append in H2.
+  apply NE_Forall_append. intuition.
+  inversion H5. assumption.
+Qed.
+
+Lemma NE_Forall_Sorted : forall x xs ys,
+  R (NE_last xs) (NE_head ys)
+    -> NE_Forall (R x) xs
+    -> NE_StronglySorted (NE_append xs ys)
+    -> NE_Forall (R x) ys.
+Proof.
+  intros.
+  induction ys; simpl in *;
+  try (constructor;
+       pose proof H1;
+       apply NE_Forall_last in H1;
+       try transitivity (NE_last xs); try assumption).
+  apply IHys.
+    apply NE_StronglySorted_inv_app in H2.
+    inversion H2. intuition. clear H4 H5.
+    inversion H7; subst.
+    apply NE_Forall_head in H8.
+    transitivity a; try assumption.
+  apply NE_StronglySorted_cons_middle with (x := a).
+  assumption.
+Qed.
+
+Fixpoint NE_StronglySorted_append (xs ys : NonEmpty A)
+  : R (NE_last xs) (NE_head ys)
+    -> NE_StronglySorted xs
+    -> NE_StronglySorted ys
+    -> NE_StronglySorted (NE_append xs ys).
+Proof.
+  intros.
+  induction xs; simpl in *.
+    constructor. assumption.
+    destruct ys; simpl in *.
+      constructor. assumption.
+    constructor. assumption.
+    apply NE_StronglySorted_inv in H2.
+    inversion H2.
+    apply NE_Forall_impl
+      with (P := R a0)
+           (Q := R a).
+      intros. transitivity a0; assumption.
+    assumption.
+  apply NE_StronglySorted_inv in H1.
+  inversion H1. intuition.
+  constructor. assumption.
+  apply NE_Forall_append.
+  intuition.
+  apply NE_Forall_Sorted with (xs := xs); assumption.
+Qed.
+
+End Sorted.
