Range.v
@@ -1,5 +1,10 @@
 Require Import Lib.
 Require Import NonEmpty.
+Require Import Hask.Alternative.
+
+Open Scope nat_scope.
+
+Import EqNotations.
 
 Generalizable All Variables.
 
@@ -14,6 +19,12 @@ Record UsePos : Set := {
   uloc   : nat;
   regReq : bool
 }.
+
+Definition upos_le (x y : UsePos) := uloc x <= uloc y.
+Definition upos_lt (x y : UsePos) := uloc x < uloc y.
+
+Program Instance upos_lt_trans : Transitive upos_lt.
+Obligation 1. unfold upos_lt in *. omega. Qed.
 
 (** ** RangeDesc *)
 
@@ -33,8 +44,12 @@ Record UsePos : Set := {
 
 Record RangeDesc := {
     rbeg : nat;
-    rend : nat;
+    rend : nat;                 (* 1 past the last use position *)
     ups  : NonEmpty UsePos;
+
+    ups_head : rbeg <= uloc (NE_head ups);
+    ups_last : uloc (NE_last ups) < rend;
+    ups_sorted : NE_StronglySorted UsePos upos_lt ups;
 
     range_nonempty : rbeg < rend         (* this comes in handy *)
 }.
@@ -49,6 +64,11 @@ Inductive Range : RangeDesc -> Prop :=
     Range {| rbeg := uloc u
            ; rend := S (uloc u)
            ; ups  := NE_Sing u
+
+           ; ups_head   := le_n (uloc u)
+           ; ups_last   := lt_n_Sn (uloc u)
+           ; ups_sorted := SSorted_sing _ _ u
+
            ; range_nonempty := le_n (S (uloc u))
            |}
 
@@ -56,13 +76,43 @@ Inductive Range : RangeDesc -> Prop :=
     Range {| rbeg := uloc u
            ; rend := rend x
            ; ups  := NE_Cons u (ups x)
+
+           ; ups_head   := le_n (uloc u)
+           ; ups_last   := ups_last x
+           ; ups_sorted := NE_StronglySorted_cons _ _ _ _
+               (lt_le_trans _ _ _ H (ups_head x)) (ups_sorted x)
+
            ; range_nonempty := Lt.lt_trans _ _ _ H (range_nonempty x)
            |}
+
+(*
+  | R_Append l r : Range l -> Range r -> forall (H : rend l <= rbeg r),
+    Range {| rbeg := rbeg l
+           ; rend := rend r
+           ; ups  := NE_append (ups l) (ups r)
+
+           ; ups_head   := eq_ind_r (fun u => rbeg l ≤ uloc u)
+                                    (ups_head l) NE_head_append_spec
+           ; ups_last   := eq_ind_r (fun u => uloc u < rend r)
+                                    (ups_last r) NE_last_append_spec
+           ; ups_sorted := NE_StronglySorted_append _ _ _ _
+                (lt_le_trans _ _ _ (ups_last l) (le_trans _ _ _ H (ups_head r)))
+                (ups_sorted l) (ups_sorted r)
+
+           ; range_nonempty :=
+               lt_le_shuffle (range_nonempty l) H (range_nonempty r)
+           |}
+*)
 
   | R_Extend x b' e' : Range x ->
     Range {| rbeg := min b' (rbeg x)
            ; rend := Peano.max e' (rend x)
            ; ups  := ups x
+
+           ; ups_head   := le_min _ _ _ (ups_head x)
+           ; ups_last   := lt_max _ _ _ (ups_last x)
+           ; ups_sorted := ups_sorted x
+
            ; range_nonempty := min_lt_max _ _ _ _ (range_nonempty x)
            |}.
 
@@ -77,7 +127,71 @@ Definition rangesIntersect `(Range x) `(Range y) : bool :=
   then rbeg y <? rend x
   else rbeg x <? rend y.
 
-Definition rangesIntersectionPoint `(xr : Range x) `(yr : Range y) : option nat :=
+Definition rangeIntersectionPoint `(xr : Range x) `(yr : Range y) : option nat :=
   if rangesIntersect xr yr
   then Some (min (rbeg x) (rbeg y))
   else None.
+
+Definition findRangeUsePos `(Range r) (f : UsePos -> bool) : option UsePos :=
+  let check u := if f u then Some u else None in
+  let fix go us := match us with
+      | NE_Sing u     => check u
+      | NE_Cons u us' => check u <|> go us'
+      end in
+  go (ups r).
+
+Fixpoint usePosSpan (f : UsePos -> bool) (l : NonEmpty UsePos)
+  : (option (NonEmpty UsePos) * option (NonEmpty UsePos)) :=
+  match l with
+    | NE_Sing u =>
+        if f u
+        then (Some l, None)
+        else (None, Some l)
+    | NE_Cons u us' =>
+        let (xl, xr) := usePosSpan f us' in
+        if f u
+        then match xl with
+               | Some xl' => (Some (NE_Cons u xl'), xr)
+               | None => (Some (NE_Sing u), xr)
+             end
+        else match xr with
+               | Some xr' => (xl, Some (NE_Cons u xr'))
+               | None => (xl, Some (NE_Sing u))
+             end
+  end.
+
+Definition rangeSpan (f : UsePos -> bool) `(r : Range rd)
+  : (option { rd1 : RangeDesc | Range rd1 } *
+     option { rd2 : RangeDesc | Range rd2 }).
+Proof.
+  destruct rd.
+  pose proof ups0 as ups1.
+  apply (usePosSpan f) in ups1.
+  destruct ups1.
+(*
+  let maybeAppend `(x : Range d) (mr : option { d : RangeDesc | Range d })
+        : option { d : RangeDesc | Range d } :=
+      match mr with
+        | Some (exist rd' r') =>
+            let res := R_Append d rd' x r' _ in
+            Some (exist _ (getRangeDesc res) res)
+        | None => Some (exist _ d x)
+      end in
+  let (xl, xr) := usePosSpan f (ups rd) in
+  let xl' := match xl with
+               | Some xl' => R_Extend (R_Sing x) (rbeg r) (rbeg r)
+  match ups rd with
+    | NE_Sing x =>
+        if f x
+        then (Some (exist _ rd r), None)
+        else (None, Some (exist _ rd r))
+    | NE_Cons x xs =>
+        let (xl, xr) := rangeSpan f xs in
+        if f x
+        then let r' :=  in
+             (maybeAppend r' xl, xr)
+        else let r' := R_Extend (R_Sing x) (rend r) (rend r) in
+             (xl, maybeAppend r' xr)
+  end.
+*)
+Admitted.
