Lib.v
@@ -135,6 +135,12 @@ Proof. intros; omega. Qed.
 Lemma lt_minus : forall n m, n > m -> n - m > 0.
 Proof. intros; omega. Qed.
 
+Lemma le_min : forall m n p, n <= p -> min m n <= p.
+Proof. intros. apply Nat.min_le_iff. right. assumption. Defined.
+
+Lemma lt_max : forall m n p, p < n -> p < max m n.
+Proof. intros. apply Nat.max_lt_iff. right. assumption. Defined.
+
 Lemma min_max_minus : forall n m b e, n - m > 0 -> Peano.max e n - min b m > 0.
 Proof.
   induction n; intros; simpl; try omega.
